src/invariant/ReorderThreadStepDiff.v
@@ -14,7 +14,7 @@ Require Import Language.
 Require Import View.
 Require Import Cell.
 Require Import Memory.
-Require Import ThreadView.
+Require Import TView.
 Require Import Thread.
 Require Import Configuration.
 
