src/opt/MergeTView.v
@@ -1,0 +1,130 @@
+Require Import Basics.
+Require Import Bool.
+Require Import List.
+
+Require Import sflib.
+Require Import paco.
+Require Import respectful5.
+
+Require Import Basic.
+Require Import Event.
+Require Import Language.
+Require Import Time.
+Require Import View.
+Require Import Cell.
+Require Import Memory.
+Require Import TView.
+Require Import Thread.
+Require Import Configuration.
+Require Import Progress.
+
+Require Import SimPromises.
+Require Import Compatibility.
+Require Import Simulation.
+
+Require Import Syntax.
+Require Import Semantics.
+
+Set Implicit Arguments.
+
+
+Lemma read_read_tview
+      loc ts released ord
+      tview0
+      (WF0: TView.wf tview0)
+      (WF_REL: View.wf released):
+  TView.le
+    (TView.read_tview (TView.read_tview tview0 loc ts released ord) loc ts released ord)
+    (TView.read_tview tview0 loc ts released ord).
+Proof.
+  econs; aggrtac;
+    (try by apply WF0);
+    repeat condtac; aggrtac.
+Qed.
+
+Lemma write_read_tview
+      loc ts ord1 ord2
+      tview0 sc0
+      (ORD: Ordering.le Ordering.seqcst ord2 -> Ordering.le Ordering.seqcst ord1)
+      (WF0: TView.wf tview0):
+  TView.le
+    (TView.read_tview (TView.write_tview tview0 sc0 loc ts ord1) loc ts
+                        ((TView.write_tview tview0 sc0 loc ts ord1).(TView.rel) loc)
+                        ord2)
+    (TView.write_tview tview0 sc0 loc ts ord1).
+Proof.
+  econs; repeat (try condtac; aggrtac; try apply WF0).
+Qed.
+
+Lemma write_write_tview
+      loc ts1 ts2 ord
+      (TS: Time.lt ts1 ts2)
+      tview0 sc0
+      (WF0: TView.wf tview0):
+  TView.le
+    (TView.write_tview (TView.write_tview tview0 sc0 loc ts1 ord)
+                         (TView.write_sc sc0 loc ts1 ord)
+                         loc ts2 ord)
+    (TView.write_tview tview0 sc0 loc ts2 ord).
+Proof.
+  econs; viewtac;
+    (repeat (condtac; aggrtac));
+    (try by apply WF0).
+  - econs; viewtac. unfold TView.write_sc. condtac; aggrtac.
+  - econs; viewtac. unfold TView.write_sc. condtac; aggrtac.
+  - econs; viewtac. unfold TView.write_sc. condtac; aggrtac.
+Qed.
+
+Lemma write_write_sc
+      loc ts1 ts2 ord
+      (TS: Time.lt ts1 ts2)
+      sc0:
+  TimeMap.le
+    (TView.write_sc (TView.write_sc sc0 loc ts1 ord)
+                     loc ts2 ord)
+    (TView.write_sc sc0 loc ts2 ord).
+Proof.
+  unfold TView.write_sc. repeat (condtac; aggrtac).
+Qed.
+
+Lemma read_fence_read_fence_tview
+      ord
+      tview0
+      (WF0: TView.wf tview0):
+  TView.le
+    (TView.read_fence_tview (TView.read_fence_tview tview0 ord) ord)
+    (TView.read_fence_tview tview0 ord).
+Proof.
+  econs; aggrtac;
+    (try by apply WF0).
+  repeat condtac; viewtac.
+Qed.
+
+Lemma write_fence_write_fence_sc
+      ord
+      tview0 sc0
+      (WF0: TView.wf tview0):
+  TimeMap.le
+    (TView.write_fence_sc (TView.write_fence_tview tview0 sc0 ord) (TView.write_fence_sc tview0 sc0 ord) ord)
+    (TView.write_fence_sc tview0 sc0 ord).
+Proof.
+  unfold TView.write_fence_tview, TView.write_fence_sc.
+  repeat (condtac; aggrtac).
+Qed.
+
+Lemma write_fence_write_fence_tview
+      ord
+      tview0 sc0
+      (WF0: TView.wf tview0):
+  TView.le
+    (TView.write_fence_tview (TView.write_fence_tview tview0 sc0 ord) (TView.write_fence_sc tview0 sc0 ord) ord)
+    (TView.write_fence_tview tview0 sc0 ord).
+Proof.
+  econs; aggrtac;
+    (try by apply WF0);
+    (repeat condtac; aggrtac);
+    rewrite <- ? View.join_r; viewtac.
+  - apply write_fence_write_fence_sc; auto.
+  - apply write_fence_write_fence_sc; auto.
+  - apply write_fence_write_fence_sc; auto.
+Qed.
