src/opt/ReorderStore.v
@@ -13,7 +13,7 @@ Require Import Time.
 Require Import View.
 Require Import Cell.
 Require Import Memory.
-Require Import ThreadView.
+Require Import TView.
 Require Import Thread.
 Require Import Configuration.
 Require Import Progress.
