src/opt/ReorderTView.v
@@ -1,0 +1,366 @@
+Require Import Basics.
+Require Import Bool.
+Require Import List.
+
+Require Import sflib.
+Require Import paco.
+Require Import respectful5.
+
+Require Import Basic.
+Require Import Event.
+Require Import Language.
+Require Import Time.
+Require Import View.
+Require Import Cell.
+Require Import Memory.
+Require Import TView.
+Require Import Thread.
+Require Import Configuration.
+Require Import Progress.
+
+Require Import SimPromises.
+Require Import Compatibility.
+Require Import Simulation.
+
+Require Import Syntax.
+Require Import Semantics.
+
+Set Implicit Arguments.
+
+
+Lemma read_read_tview
+      loc1 ts1 released1 ord1
+      loc2 ts2 released2 ord2
+      tview0
+      (WF0: TView.wf tview0)
+      (WF1: View.wf released1)
+      (WF2: View.wf released2):
+  TView.le
+    (TView.read_tview
+       (TView.read_tview tview0 loc2 ts2 released2 ord2)
+       loc1 ts1 released1 ord1)
+    (TView.read_tview
+       (TView.read_tview tview0 loc1 ts1 released1 ord1)
+       loc2 ts2 released2 ord2).
+Proof.
+  econs; aggrtac;
+    (try by apply WF0);
+    (try by condtac; aggrtac).
+Qed.
+
+Lemma read_write_tview
+      loc1 ts1 released1 ord1
+      loc2 ts2 ord2
+      tview0 sc0
+      (WF0: TView.wf tview0)
+      (WF1: View.wf released1):
+  TView.le
+    (TView.read_tview
+       (TView.write_tview tview0 sc0 loc2 ts2 ord2)
+       loc1 ts1 released1 ord1)
+    (TView.write_tview
+       (TView.read_tview tview0 loc1 ts1 released1 ord1)
+       sc0 loc2 ts2 ord2).
+Proof.
+  econs; aggrtac;
+    (try by apply WF0);
+    (try by condtac; aggrtac).
+  repeat condtac; aggrtac; try apply WF0.
+Qed.
+
+Lemma read_read_fence_tview
+      loc1 ts1 released1 ord1
+      ord2
+      tview0
+      (WF0: TView.wf tview0)
+      (WF1: View.wf released1):
+  TView.le
+    (TView.read_tview
+       (TView.read_fence_tview tview0 ord2)
+       loc1 ts1 released1 ord1)
+    (TView.read_fence_tview
+       (TView.read_tview tview0 loc1 ts1 released1 ord1)
+       ord2).
+Proof.
+  econs; aggrtac;
+    (try by apply WF0);
+    (try by condtac; aggrtac).
+  - repeat condtac; aggrtac; try apply WF0.
+  - repeat condtac; aggrtac; try apply WF0.
+    destruct ord1; inv COND; inv COND1.
+Qed.
+
+Lemma read_write_fence_tview
+      loc1 ts1 released1 ord1
+      ord2
+      tview0 sc0
+      (WF0: TView.wf tview0)
+      (WF1: View.wf released1):
+  TView.le
+    (TView.read_tview
+       (TView.write_fence_tview tview0 sc0 ord2)
+       loc1 ts1 released1 ord1)
+    (TView.write_fence_tview
+       (TView.read_tview tview0 loc1 ts1 released1 ord1)
+       sc0 ord2).
+Proof.
+  unfold TView.write_fence_tview, TView.write_fence_sc.
+  econs; repeat (try condtac; aggrtac; try apply WF0).
+Qed.
+
+Lemma write_read_tview
+      loc1 ts1 ord1
+      loc2 ts2 released2 ord2
+      tview0 sc0
+      (ORD1: Ordering.le ord1 Ordering.relaxed)
+      (WF0: TView.wf tview0)
+      (WF2: View.wf released2):
+  TView.le
+    (TView.write_tview
+       (TView.read_tview tview0 loc2 ts2 released2 ord2)
+       sc0 loc1 ts1 ord1)
+    (TView.read_tview
+       (TView.write_tview tview0 sc0 loc1 ts1 ord1)
+       loc2 ts2 released2 ord2).
+Proof.
+  econs; aggrtac;
+    (try by apply WF0);
+    (try by condtac; aggrtac).
+  condtac; aggrtac. condtac.
+  - destruct ord1; inv ORD1; inv COND0.
+  - aggrtac; try apply WF0.
+Qed.
+
+Lemma write_write_tview
+      loc1 ts1 ord1
+      loc2 ts2 ord2
+      tview0 sc0
+      (ORD1: Ordering.le ord1 Ordering.relaxed)
+      (WF0: TView.wf tview0):
+  TView.le
+    (TView.write_tview
+       (TView.write_tview tview0 sc0 loc2 ts2 ord2)
+       (TView.write_sc sc0 loc2 ts2 ord2)
+       loc1 ts1 ord1)
+    (TView.write_tview
+       (TView.write_tview tview0 sc0 loc1 ts1 ord1)
+       (TView.write_sc sc0 loc1 ts1 ord1)
+       loc2 ts2 ord2).
+Proof.
+  econs; aggrtac;
+    (try by apply WF0);
+    (repeat (condtac; aggrtac; try apply WF0)).
+  - rewrite <- ? View.join_r.
+    econs; aggrtac. apply TViewFacts.write_sc_incr.
+  - rewrite <- ? View.join_r.
+    econs; aggrtac. apply TViewFacts.write_sc_incr.
+  - rewrite <- ? View.join_r.
+    econs; aggrtac. apply TViewFacts.write_sc_incr.
+  - econs; viewtac.
+    rewrite <- ? TimeMap.join_r.
+    apply TViewFacts.write_sc_incr.
+Qed.
+
+Lemma write_write_sc
+      loc1 ts1 ord1
+      loc2 ts2 ord2
+      sc0
+      (LOC: loc1 <> loc2)
+      (ORD1: Ordering.le ord1 Ordering.relaxed):
+  TimeMap.le
+    (TView.write_sc
+       (TView.write_sc sc0 loc2 ts2 ord2)
+       loc1 ts1 ord1)
+    (TView.write_sc
+       (TView.write_sc sc0 loc1 ts1 ord1)
+       loc2 ts2 ord2).
+Proof.
+  ii. unfold TView.write_sc. aggrtac.
+Qed.
+
+Lemma write_read_fence_tview
+      loc1 ts1 ord1
+      ord2
+      tview0 sc0
+      (ORD2: Ordering.le ord2 Ordering.relaxed)
+      (WF0: TView.wf tview0):
+  TView.le
+    (TView.write_tview
+       (TView.read_fence_tview tview0 ord2)
+       sc0 loc1 ts1 ord1)
+    (TView.read_fence_tview
+       (TView.write_tview tview0 sc0 loc1 ts1 ord1)
+       ord2).
+Proof.
+  econs; repeat (try condtac; aggrtac; try apply WF0).
+Qed.
+
+Lemma write_write_fence_tview
+      loc1 ts1 ord1
+      ord2
+      tview0 sc0
+      (ORD2: Ordering.le ord2 Ordering.acqrel)
+      (WF0: TView.wf tview0):
+  TView.le
+    (TView.write_tview
+       (TView.write_fence_tview tview0 sc0 ord2)
+       (TView.write_fence_sc tview0 sc0 ord2)
+       loc1 ts1 ord1)
+    (TView.write_fence_tview
+       (TView.write_tview tview0 sc0 loc1 ts1 ord1)
+       (TView.write_sc sc0 loc1 ts1 ord1)
+       ord2).
+Proof.
+  unfold TView.write_fence_tview, TView.write_fence_sc.
+  econs; repeat (try condtac; aggrtac; try apply WF0).
+Qed.
+
+Lemma read_fence_read_tview
+      ord1
+      loc2 ts2 released2 ord2
+      tview0
+      (ORD2: Ordering.le ord2 Ordering.unordered \/ Ordering.le Ordering.acqrel ord2)
+      (WF0: TView.wf tview0):
+  TView.le
+    (TView.read_fence_tview
+       (TView.read_tview tview0 loc2 ts2 released2 ord2)
+       ord1)
+    (TView.read_tview
+       (TView.read_fence_tview tview0 ord1)
+       loc2 ts2 released2 ord2).
+Proof.
+  econs; repeat (try condtac; aggrtac; try apply WF0).
+  des; [|congr]. destruct ord2; inv ORD2; inv COND0.
+Qed.
+
+Lemma read_fence_write_tview
+      ord1
+      loc2 ts2 ord2
+      tview0 sc0
+      (WF0: TView.wf tview0):
+  TView.le
+    (TView.read_fence_tview
+       (TView.write_tview tview0 sc0 loc2 ts2 ord2)
+       ord1)
+    (TView.write_tview
+       (TView.read_fence_tview tview0 ord1)
+       sc0 loc2 ts2 ord2).
+Proof.
+  econs; repeat (try condtac; aggrtac; try apply WF0).
+Qed.
+
+Lemma write_fence_read_tview
+      ord1
+      loc2 ts2 released2 ord2
+      tview0 sc0
+      (ORD1: Ordering.le ord1 Ordering.relaxed)
+      (WF0: TView.wf tview0)
+      (WF2: View.wf released2):
+  TView.le
+    (TView.write_fence_tview
+       (TView.read_tview tview0 loc2 ts2 released2 ord2) sc0 ord1)
+    (TView.read_tview
+       (TView.write_fence_tview tview0 sc0 ord1)
+       loc2 ts2 released2 ord2).
+Proof.
+  econs; aggrtac;
+    (try by apply WF0);
+    (repeat (condtac; aggrtac; try apply WF0)).
+Qed.
+
+Lemma write_fence_read_sc
+      ord1
+      loc2 ts2 released2 ord2
+      tview0 sc0
+      (ORD1: Ordering.le ord1 Ordering.relaxed)
+      (WF0: TView.wf tview0):
+  TimeMap.le
+    (TView.write_fence_sc
+       (TView.read_tview tview0 loc2 ts2 released2 ord2) sc0 ord1)
+    (TView.write_fence_sc tview0 sc0 ord1).
+Proof.
+  ii. unfold TView.write_sc, TView.write_fence_sc.
+  repeat condtac; aggrtac.
+Qed.
+
+Lemma write_fence_write_tview
+      ord1
+      loc2 ts2 ord2
+      tview0 sc0
+      (ORD1: Ordering.le ord1 Ordering.relaxed)
+      (WF0: TView.wf tview0):
+  TView.le
+    (TView.write_fence_tview
+       (TView.write_tview tview0 sc0 loc2 ts2 ord2)
+       (TView.write_sc sc0 loc2 ts2 ord2)
+       ord1)
+    (TView.write_tview
+       (TView.write_fence_tview tview0 sc0 ord1)
+       sc0 loc2 ts2 ord2).
+Proof.
+  econs; aggrtac;
+    (try by apply WF0);
+    (repeat (condtac; aggrtac; try apply WF0)).
+Qed.
+
+Lemma write_fence_write_sc
+      ord1
+      loc2 ts2 ord2
+      tview0 sc0
+      (ORD1: Ordering.le ord1 Ordering.relaxed)
+      (WF0: TView.wf tview0):
+  TimeMap.le
+    (TView.write_fence_sc
+       (TView.write_tview tview0 sc0 loc2 ts2 ord2)
+       (TView.write_sc sc0 loc2 ts2 ord2)
+       ord1)
+    (TView.write_sc
+       (TView.write_fence_sc tview0 sc0 ord1)
+       loc2 ts2 ord2).
+Proof.
+  ii. unfold TView.write_sc, TView.write_fence_sc.
+  repeat condtac; aggrtac.
+Qed.
+
+Lemma read_fence_write_fence_tview
+      ord1
+      ord2
+      tview0 sc0
+      (WF0: TView.wf tview0):
+  TView.le
+    (TView.read_fence_tview
+       (TView.write_fence_tview tview0 sc0 ord2)
+       ord1)
+    (TView.write_fence_tview
+       (TView.read_fence_tview tview0 ord1)
+       sc0 ord2).
+Proof.
+  unfold TView.write_fence_tview, TView.write_fence_sc.
+  econs; repeat (try condtac; aggrtac; try apply WF0).
+  - rewrite <- TimeMap.join_r. apply WF0.
+  - rewrite <- TimeMap.join_r. apply WF0.
+  - rewrite <- TimeMap.join_r. apply WF0.
+  - rewrite <- View.join_r. viewtac.
+    rewrite <- TimeMap.join_r. apply WF0.
+  - rewrite <- View.join_r. viewtac.
+    rewrite <- TimeMap.join_r. apply WF0.
+Qed.
+
+Lemma read_write_tview_eq
+      loc1 ts1 released1 ord1
+      loc2 ts2 ord2
+      tview0 sc0
+      (ORD1: Ordering.le ord2 Ordering.relaxed)
+      (WF0: TView.wf tview0)
+      (WF1: View.wf released1):
+  (TView.read_tview
+     (TView.write_tview tview0 sc0 loc2 ts2 ord2)
+     loc1 ts1 released1 ord1) =
+  (TView.write_tview
+     (TView.read_tview tview0 loc1 ts1 released1 ord1)
+     sc0 loc2 ts2 ord2).
+Proof.
+  apply TView.antisym.
+  - apply read_write_tview; auto.
+  - apply write_read_tview; auto.
+Qed.
